
 	

| Name of rule        | Rule                                                                       | Example                                                                                                    |
| ------------------- | -------------------------------------------------------------------------- | ---------------------------------------------------------------------------------------------------------- |
| Product of power    | Add powers together when multiplying like bases                            | a<sup>n</sup> × a<sup>m</sup> = a<sup>m+n</sup> => a<sup>2</sup> × a<sup>4</sup> = a<sup>6</sup>           |
| Quotient of powers  | Subtract powers when dividing like bases                                   | a<sup>m</sup> ÷ a<sup>n</sup> = a<sup>m-n</sup> => a<sup>5</sup> ÷ a<sup>3</sup> = a<sup>2</sup>           |
| Power of a power    | Multiply powers together when raising a power by another exponent          | (a<sup>m</sup>)<sup>n</sup> = a<sup>mn</sup> => (a<sup>3</sup>)<sup>4</sup> =  a<sup>12</sup>              |
| Power of a product  | Distribute power to each base when raising several variables by a power    | (ab)<sup>m</sup> = a<sup>m</sup> × b<sup>m</sup> => (ab)<sup>m</sup> = a<sup>8</sup> × b<sup>8</sup>       |
| Power of a quotient | Distribute power to all values in a quotient                               | (a/b)<sup>m</sup> = a<sup>m</sup> / b<sup>m</sup> => (1/3)<sup>2</sup> = 1<sup>2</sup>/3<sup>2</sup> = 1/9 |
| Zero power          | Any base raised to the power of zero becomes one                           | a<sup>0</sup> = 1                                                                                          |
| Negative exponent   | To change a negative exponent to a positive one, flip it into a reciprocal | a<sup>-m</sup> = 1/a<sup>m</sup> => a<sup>-8</sup> = 1/a<sup>8</sup>                                       |
